@prefix rdf: <http://www.w3.org/1999/02/22-rdf-syntax-ns#> .
@prefix rdfs: <http://www.w3.org/2000/01/rdf-schema#> .
@prefix owl: <http://www.w3.org/2002/07/owl#> .
@prefix xsd: <http://www.w3.org/2001/XMLSchema#> .
@prefix skos: <http://www.w3.org/2004/02/skos/core#> .
@prefix dcterms: <http://purl.org/dc/terms/> .
@prefix foaf: <http://xmlns.com/foaf/0.1/>.
@prefix vann: <http://purl.org/vocab/vann/> .
@prefix voaf: <http://purl.org/vocommons/voaf#> .
@prefix time: <http://www.w3.org/2006/time#> .

@prefix schema: <http://schema.org/> .

@prefix sosa: <http://www.w3.org/ns/sosa/> .
@prefix sosa-systems: <http://www.w3.org/ns/sosa/systems/> .


sosa-systems: a owl:Ontology , voaf:Vocabulary ;
  dcterms:title "Ontology of operating conditions and capabilities of systems"@en ;
  dcterms:description "The System Capabilities Module imports SOSA and adds classes and properties required for the description of the operating conditions and capabilities of systems, particularly Sensors and Actuators."@en ;
  dcterms:creator [ a foaf:Agent ; foaf:name "W3C/OGC Spatio-temporal Data on the Web Working Group"@en ] ;
  dcterms:rights "Copyright 2025 W3C/OGC." ;
  dcterms:license <http://www.w3.org/Consortium/Legal/2015/copyright-software-and-document> ;
  dcterms:license <http://www.opengeospatial.org/ogc/Software> ;
  rdfs:comment "Please report any errors to the W3C Spatio-temporal Data on the Web Working Group via the SDW WG Public List public-sdw-wg@w3.org"@en ;
  rdfs:seeAlso <https://www.w3.org/2015/spatial/wiki/Semantic_Sensor_Network_Ontology> ;
  dcterms:created "2017-05-14"^^xsd:date ;
  dcterms:modified "2025-06-24"^^xsd:date ;
  vann:preferredNamespacePrefix "sosa" ;
  vann:preferredNamespaceUri "http://www.w3.org/ns/sosa/" ;
  owl:imports sosa: .

## Classes and relationships involved in the description of the operating conditions of a system (typically an observation collection about the system environment).

sosa:hasOperatingConditions
  a owl:ObjectProperty ;
  rdfs:label "has operating conditions"@en ;
  skos:definition """
  Relation between a System and an ObservationCollection (or Observation) describing conditions under which the System operates more or less normally (TODO improve here). A short but extensible list of operating condition kinds is provided in SSN-System, such as normal operating conditions, suboptimal conditions, and survivable conditions.
  """@en ;
  schema:domainIncludes sosa:System ;
  schema:rangeIncludes sosa:ObservationCollection , sosa:Observation ;
  rdfs:isDefinedBy sosa-systems: .


sosa:hasOperatingConditionKind
  a owl:ObjectProperty ;
  rdfs:label "has operating condition kind"@en ;
  skos:definition """
  Relation between an ObservationCollection (or Observation) and an OperatingConditionKind describing the kind of the operating conditions in the context of the system. A short but extensible list of operating condition kinds is provided in SSN-System, such as normal operating conditions, suboptimal conditions, and survivable conditions.
  """@en ;
  schema:domainIncludes sosa:ObservationCollection , sosa:Observation ;
  schema:rangeIncludes sosa:OperatingConditionKind ;
  rdfs:isDefinedBy sosa-systems: .

sosa:OperatingConditionKind a owl:Class ;
  rdfs:label "Operating Condition Kind"@en ;
  skos:definition """
  A concept that describes the kind of operating conditions in the context of a system. A short but extensible list of operating condition kinds is provided in SSN-System, such as normal operating conditions, suboptimal conditions, and survivable conditions.
  """@en ;
  rdfs:subClassOf skos:Concept ;
  rdfs:isDefinedBy sosa-systems: .

## A short but extensible list of operating condition kinds is provided in SSN-System, such as normal operating conditions, suboptimal conditions, and survivable conditions.

sosa:NormalOperatingConditions rdfs:subClassOf sosa:OperatingConditionKind ;
  rdfs:label "Normal Operating Conditions"@en ;
  skos:definition """
  The conditions under which a system is expected to operate normally.
  """@en ;
  rdfs:isDefinedBy sosa-systems: .

sosa:SuboptimalOperatingConditions rdfs:subClassOf sosa:OperatingConditionKind ;
  rdfs:label "Suboptimal Conditions"@en ;
  skos:definition """
  The conditions under which a system is expected to operate suboptimally, but may recover if the conditions are restored to normal operating conditions.
  """@en ;
  rdfs:isDefinedBy sosa-systems: .

sosa:SurvivableConditions rdfs:subClassOf sosa:OperatingConditionKind ;
  rdfs:label "Survivable Conditions"@en ;
  skos:definition """
  The conditions under which a system is expected to survive. The system may be damaged if the survivable conditions are violated.
  """@en ;
  rdfs:isDefinedBy sosa-systems: .

## Relationship involved in the description of the System capability

sosa:hasSystemCapability a owl:ObjectProperty ;
  schema:domainIncludes sosa:System , sosa:Sensor, sosa:Actuator, sosa:Sampler ;
  schema:rangeIncludes sosa:ExecutionCollection , sosa:Execution ;
  rdfs:label "has system capability"en ;
  skos:definition "Relation between a System and an ObservationCollection (or Observation) describing the capability of the system. A sensor or system may have more than one set of system capabilities that are related to the conditions under which they hold true."@en ;
  rdfs:isDefinedBy sosa-systems: .
  

## Detailed classes and relationships involved in the description of the conditions (typically an observation collection about the system environment) under which an observation or property (typically about the system capabilities) is valid

sosa:inCondition a owl:ObjectProperty ;
  schema:domainIncludes sosa:Observation , sosa:Property ;
  schema:rangeIncludes sosa:ExecutionCollection , sosa:Execution ;
  rdfs:label "in condition"@en ;
  skos:definition "Describes the conditions (typically an observation collection about the system environment) defining the validity context of an observation (typically about the system capabilities) or a property (typically about the system capabilities)."@en ;
  rdfs:isDefinedBy sosa-systems: .


## Battery
sosa:Battery rdfs:subClassOf sosa:System ;
  rdfs:label "Battery"@en ;
  skos:definition """
  A Battery powering a System as its primary or secondary power source. As this is a specialization of the System class modeling of integrated battery management systems is also possible.
  """@en ;
  rdfs:isDefinedBy sosa-systems: .

ssn:BatteryLifetime a owl:Class ;
  rdfs:label "Battery Lifetime"@en ;
  skos:definition "Total useful life of a battery."@en ;
  rdfs:subClassOf sosa:Property ;
  rdfs:isDefinedBy sosa-systems: .
