@prefix rdf: <http://www.w3.org/1999/02/22-rdf-syntax-ns#> .
@prefix rdfs: <http://www.w3.org/2000/01/rdf-schema#> .
@prefix owl: <http://www.w3.org/2002/07/owl#> .
@prefix xsd: <http://www.w3.org/2001/XMLSchema#> .
@prefix skos: <http://www.w3.org/2004/02/skos/core#> .
@prefix dcterms: <http://purl.org/dc/terms/> .
@prefix foaf: <http://xmlns.com/foaf/0.1/>.
@prefix time: <http://www.w3.org/2006/time#> .

@prefix schema: <http://schema.org/> .

@prefix sosa: <http://www.w3.org/ns/sosa/> .
@prefix sosa-common: <http://www.w3.org/ns/sosa/common/> .


sosa-common: 
  a owl:Ontology ;
  dcterms:title "Sensor, Observation, Sample, and Actuator (SOSA) Ontology - core module"@en ;
  dcterms:description "Core classes and properties for the SSN Ontology."@en ;
  dcterms:creator [ a foaf:Agent ; foaf:name "W3C/OGC Spatial Data on the Web Working Group"@en ] ;
  dcterms:rights "Copyright 2025 W3C/OGC." ;
  dcterms:license <http://www.w3.org/Consortium/Legal/2015/copyright-software-and-document> ;
  dcterms:license <http://www.opengeospatial.org/ogc/Software> ;
  dcterms:created "2024-02-02"^^xsd:date ;
  .


## Features of interest and Property

sosa:FeatureOfInterest 
  a owl:Class ;
  rdfs:label "Feature Of Interest"@en ;
  skos:definition """
  entity that is the target of an Execution or Deployment

  i.e., whose property is being estimated by an Observation, 
  or whose property is being manipulated by an Actuator, 
  or which is being sampled or transformed in an act of Sampling, 
  or which is the target of Executions planned as part of a Deployment.
  """@en ;
  skos:example "When measuring the height of a tree, the height is the observed Property, 20m may be the Result of the Observation, and the tree is the FeatureOfInterest. A window is a FeatureOfInterest for an automatic window control Actuation."@en ;
  rdfs:isDefinedBy sosa-common: .

sosa:Property 
  a owl:Class ;
  rdfs:label "Property"@en ;
  skos:definition """
  identifiable quality of features of interest that can be observed or acted upon

  A property can apply to different features of interest.

  """@en ;
  skos:example "Cars (a feature type) all have a characteristic colour, where 'colour' is a property."@en ;
  skos:note "Concepts from existing code lists, vocabularies, and taxonomies, may be used as instances of Property"@en ;
  rdfs:isDefinedBy sosa-common: .

sosa:forProperty 
  a owl:ObjectProperty ;
  rdfs:label "for property"@en ;
  skos:definition """
  relation from some Procedure or System to a Property it acts on or observes
  """@en ;
  skos:example "For example, from a Sensor to the properties it can observe; from an Actuator to the properties it can act on; from a SystemCapability to the Property the capability is described for."@en ;
  schema:domainIncludes sosa:Procedure ;
  schema:domainIncludes sosa:System ;
  schema:rangeIncludes sosa:Property ;
  rdfs:isDefinedBy sosa-common: .

sosa:hasProperty 
  a owl:ObjectProperty ; 
  rdfs:label "has property"@en ;
  skos:definition """
  relation from an entity to a Property of that entity
  """@en ;
  schema:domainIncludes sosa:FeatureOfInterest ;
  schema:rangeIncludes sosa:Property ;
  owl:inverseOf sosa:isPropertyOf ;
  rdfs:isDefinedBy sosa-common: .

sosa:isFeatureOfInterestOf 
  a owl:ObjectProperty ;
  rdfs:label "is feature of interest of"@en ;
  skos:definition """
  relation from a FeatureOfInterest to an Execution, Execution Collection, or Deployment, operating on it

  i.e., to an Observation about it, to an Actuation acting on it, to an act of Sampling that sampled it,
  or to a Deployment for which it is the subject.
"""@en ;
  schema:domainIncludes sosa:FeatureOfInterest ;
  schema:rangeIncludes sosa:Deployment ;
  schema:rangeIncludes sosa:Execution ;
  schema:rangeIncludes sosa:ExecutionCollection ;
  owl:inverseOf sosa:hasFeatureOfInterest ;
  rdfs:isDefinedBy sosa-common: .

sosa:isPropertyOf 
  a owl:ObjectProperty ;
  rdfs:label "is property of"@en ;
  skos:definition """
  relation from a Property to a FeatureOfInterest that it is a quality of
  """@en ;
  schema:domainIncludes sosa:Property ;
  schema:rangeIncludes sosa:FeatureOfInterest ;
  owl:inverseOf sosa:hasProperty ; 
  rdfs:isDefinedBy sosa-common: .

sosa:isUltimateFeatureOfInterestOf 
  a owl:ObjectProperty ;
  rdfs:label "is ultimate feature of interest of"@en ;
  skos:definition """
  relation from an ultimate FeatureOfInterest to an Execution, ExecutionCollection, or Deployment, for which it is the ultimate subject
  """@en ;
  schema:domainIncludes sosa:FeatureOfInterest ;
  schema:rangeIncludes sosa:Deployment ;
  schema:rangeIncludes sosa:Execution ;
  schema:rangeIncludes sosa:ExecutionCollection ;
  owl:inverseOf sosa:hasUltimateFeatureOfInterest ;
  rdfs:isDefinedBy sosa-common: .

sosa:propertyFor 
  a owl:ObjectProperty ;
  rdfs:label "property for"@en ;
  skos:definition """
  relation from a Property to some Procedure or System that acts on it or observes it
  """@en ;
  skos:example "For example, from a Sensor to the properties it can observe; from an Actuator to the properties it can act on; from a SystemCapability to the Property the capability is described for."@en ;
  schema:domainIncludes sosa:Property ;
  schema:rangeIncludes sosa:Procedure ;
  schema:rangeIncludes sosa:System ;
  rdfs:isDefinedBy sosa-common: .


## Procedures

sosa:Procedure 
  a owl:Class ;
  rdfs:label "Procedure"@en ;
  skos:definition """
  workflow, protocol, plan, algorithm, or computational method specifying how to make an Execution

  A Procedure is re-usable, and might be applied in many Actuations, Observations, or Samplings.
  It explains the steps to be carried out to arrive at reproducible results.
  """@en ;
  skos:example "The measured wind speed differs depending on the height of the sensor above the surface, e.g., due to friction. Consequently, procedures for measuring wind speed define a standard height for anemometers above ground, typically 10m for meteorological measures and 2m in Agrometeorology. This definition of height, sensor placement, and so forth are defined by the Procedure."@en ;
  skos:scopeNote """
  Procedure generalizes the ActuationProcedure, ObservationProcedure, and SamplingProcedure classes. 
  It appears in the ontology to support the description of a common pattern for executions and their properties. 
  """@en ;
  rdfs:isDefinedBy sosa-common: .

sosa:hasInput 
  a owl:ObjectProperty ;
  rdfs:label "has input"@en ;
  skos:definition """
  relation from a Procedure to an input required for its execution
  """@en ;
  skos:scopeNote "An input might be a calibration or conditioning parameter, or the output of a previous procedure within an extended processing chain."@en ;
  skos:note "This property will typically describe the type of the inputs required to execute the Procedure."@en ;
  schema:domainIncludes sosa:Procedure ;
  owl:inverseOf sosa:inputFor ;
  rdfs:isDefinedBy sosa-common: .

sosa:hasOutput 
  a owl:ObjectProperty ;
  rdfs:label "has output"@en ;
  skos:definition """
  relation from a Procedure to an output or result of its execution
  """@en ;
  skos:note "This property will typically describe the type of the result from executing the Procedure."@en ;
  schema:domainIncludes sosa:Procedure ;
  owl:inverseOf sosa:outputFor ;
  rdfs:isDefinedBy sosa-common: .

sosa:hasProcedure 
  a owl:ObjectProperty ;
  rdfs:label "has procedure"@en ;
  skos:definition """
  relation from a Property to a Procedure that can observe or act on it
  """@en ;
  schema:domainIncludes sosa:Property ;
  schema:rangeIncludes sosa:Procedure ;
  rdfs:isDefinedBy sosa-common: .

sosa:implementedBy 
  a owl:ObjectProperty ;
  rdfs:label "implemented by"@en ;
  skos:definition """
  relation from a Procedure to a System that implements it
  """@en ;
  skos:example "For example, the relationship between a scientific measuring Procedure and a sensor that senses via that Procedure."@en ;
  schema:domainIncludes sosa:Procedure ;
  schema:rangeIncludes sosa:System ;
  owl:inverseOf sosa:implements ;
  rdfs:isDefinedBy sosa-common: .

sosa:inputFor 
  a owl:ObjectProperty ;
  rdfs:label "input for"@en ;
  skos:definition """
  relation from an input to a Procedure that uses it in an Execution
  """@en ;
  schema:rangeIncludes sosa:Procedure ;
  owl:inverseOf sosa:hasInput ;
  rdfs:isDefinedBy sosa-common: .

sosa:outputFor 
  a owl:ObjectProperty ;
  rdfs:label "output for"@en ;
  skos:definition """
  relation from an output or result to a Procedure that generates it in an Execution
  """@en ;
  schema:rangeIncludes sosa:Procedure ;
  owl:inverseOf sosa:hasOutput ;
  rdfs:isDefinedBy sosa-common: .

sosa:usedForExecution 
  a owl:ObjectProperty ;
  rdfs:label "used for execution"@en ;
  skos:definition """
  relation from a Procedure to an Execution made using it
  """@en ;
  schema:domainIncludes sosa:Procedure ;
  schema:rangeIncludes sosa:Execution ;
  owl:inverseOf sosa:usedProcedure ;
  rdfs:isDefinedBy sosa-common: .

## Executions

sosa:Execution 
  a owl:Class ;
  rdfs:label "Execution of a Procedure"@en ;
  skos:definition """
  act of carrying out a Procedure using a System
  """@en ;
  skos:scopeNote """
  Execution generalizes the Actuation, Observation, and Sampling classes. 
  It appears in the ontology to support the description of a common pattern for executions and their properties. 

  Execution MUST be considered to be abstract, so any individual Execution SHOULD be declared to be an instance of one of the concrete sub-classes, and not of the Execution class.
  """@en ;
  rdfs:isDefinedBy sosa-common: .

sosa:ExecutionCollection 
  a owl:Class ;
  rdfs:label "Execution Collection"@en ;
  skos:definition """
  set of one or more Executions or ExecutionCollections; collections may be nested

  The following execution properties may appear in an Execution Collection: 
  hasFeatureOfInterest , usedProcedure , madeBySystem , endTime, resultTime , startTime . 
  If it is present, the value of a property summarizes the values of the matching properties of the member executions, where membership is either direct or transitive through one or more member execution collections. 
  The following consistency rules apply with respect to the execution properties listed above: 
  
  1. Where an individual Execution Collection omits a property, a member Execution (direct or transitive) MAY have any value for that property.

  2. Where an individual Execution Collection has a single value for a property, each member Execution (direct or transitive) MUST have that same value for the property - i.e., the collection is homogeneous in that property.  That property MAY then be omitted in any member Observation or Observation Collection.

  3. Where an individual Execution Collection has more than one value for a property, each member Execution (direct or transitive) MUST have a value for that property that matches one of the values for the property in the collection. 
  
  4. Where an individual Execution Collection has a value for a property that is a range or interval, each member Execution (direct or transitive) MUST have a value for that property that matches or falls within that range or interval.

  5. Where an individual Execution Collection has more than one value for a property that is a range or interval, each member Execution (direct or transitive) MUST have a value for that property that either matches or falls within one of those ranges or intervals.
  """@en ;
  skos:note """The members of a collection do not necessarily share a common value for any property. """@en ;
  skos:scopeNote """
  Execution Collection generalizes the Actuation Collection, Observation Collection, and Sampling Collection classes. 
  It appears in the ontology to support the description of a common pattern for executions and their properties. 

  Execution Collection MUST be considered to be abstract, so any individual Execution Collection SHOULD be declared to be an instance of one of the concrete sub-classes, and not of the Execution Collection class.
  """@en ;
  rdfs:isDefinedBy sosa-common: .

sosa:Result 
  a owl:Class ;
  owl:deprecated true ;
  rdfs:label "Result"@en ;
  skos:definition """
  outcome of an Observation, Actuation, or act of Sampling. 
  
  To store an observation's simple result value one can use the hasSimpleResult property.
  """@en ;
  skos:example "The value 20 as the height of a certain tree together with the unit, e.g., Meter."@en ;
  rdfs:isDefinedBy sosa-common: .

sosa:endTime 
  a owl:DatatypeProperty ;
  rdfs:label "end time"@en ;
  skos:definition """
  instant of time when the Execution or ExecutionCollection or Deployment was ended or completed
  """@en ;
  rdfs:comment "The value would usually be encoded using xsd:dateTime xsd:date xsd:gYearMonth xsd:gYear"@en ;
  schema:domainIncludes sosa:Execution ;
  schema:domainIncludes sosa:ExecutionCollection ;
  schema:domainIncludes sosa:Deployment ;
  rdfs:isDefinedBy sosa-common: .

sosa:hasFeatureOfInterest 
  a owl:ObjectProperty ;
  rdfs:label "has feature of interest"@en ;
  skos:definition """
  relation from an Execution, Execution Collection, or Deployment, to its subject entity

  i.e., from an Actuation to the entity whose property was modified;
  from an Observation to the entity whose quality was observed;
  from an act of Sampling to the entity that was sampled;
  or from a Deployment to its target
  """@en ;
  skos:scopeNote "This is the _proximate_ feature of interest, which may be a proxy entity such as a sample of the _ultimate_ feature of interest. Use `hasUltimateFeatureOfInterest` if the intention is to link to the _ultimate_ feature of interest. " ;
  skos:example "For example, in an Observation of the weight of a person, the FeatureOfInterest is the person and the property is its weight."@en ;
  schema:domainIncludes sosa:Deployment ;
  schema:domainIncludes sosa:Execution ;
  schema:domainIncludes sosa:ExecutionCollection ;
  schema:rangeIncludes sosa:FeatureOfInterest ;
  owl:inverseOf sosa:isFeatureOfInterestOf ;
  rdfs:isDefinedBy sosa-common: .

sosa:hasInputValue 
  a owl:ObjectProperty ;
  rdfs:label "has input value"@en ;
  skos:definition """
  assigns a value to an input defined by the Procedure that is used in an Execution
  """@en ;
  skos:note "The input value MUST be consistent with a hasInput definition from the corresponding Procedure"@en ;
  skos:scopeNote "The input might be a calibration or conditioning parameter, or the result of a previous execution within an extended processing chain."@en ;
  schema:domainIncludes sosa:Execution ;
  rdfs:isDefinedBy sosa-common: .

sosa:hasResult 
  a owl:ObjectProperty ;
  rdfs:label "has result"@en ;
  skos:definition """
  relation from an Execution to its result

  In the case of an Actuation, the result is the expected value of the Property following the execution of the Procedure by the Actuator. 

  In the case of an Observation, the result is the value of the Property produced by the execution of the Procedure by the Sensor. 
  
  In the case of a Sampling, the result is the Sample produced by the execution of the Procedure by the Sampler. 

  An Execution has a single result, therefore sosa:hasResult is Functional.
  """@en ;
  skos:note "The result value MUST be consistent with the hasOutput definition from the corresponding Procedure"@en ;
  schema:domainIncludes sosa:Execution ;
  schema:domainIncludes sosa:ExecutionCollection ;
  owl:inverseOf sosa:isResultOf ;
  rdfs:isDefinedBy sosa-common: .

sosa:hasSimpleResult 
  a owl:DatatypeProperty ;
  rdfs:label "has simple result"@en ;
  skos:definition """
  relation from an Execution to its simple value

  In the case of an Actuation, the result is the expected value of the Property following the execution of the Procedure by the Actuator. 

  In the case of an Observation, the result is the value of the Property produced by the execution of the Procedure by the Sensor. 
  """@en ;
  skos:example "For instance, the values 23 or true."@en ;
  skos:note "This DatatypeProperty provides an alternative to hasResult, to be used only if the execution result can be expressed as a Literal"@en ;
  schema:domainIncludes sosa:Execution ;
  schema:domainIncludes sosa:ExecutionCollection ;
  rdfs:isDefinedBy sosa-common: .

sosa:hasUltimateFeatureOfInterest 
  a owl:ObjectProperty ;
  rdfs:label "has ultimate feature of interest"@en  ;
  skos:definition """
  relation from an Execution to its ultimate subject entity

  i.e., from an Actuation to the ultimate entity whose property was modified;
  from an Observation to the ultimate entity whose quality was observed;
  from an act of Sampling to the ultimate entity that was sampled;
  or from a Deployment to its ultimate target
  """@en ;
  skos:scopeNote "This is useful when the proximate feature of interest is a sample of the ultimate feature of interest, directly or transitively." ;
  skos:note """should match a property chain something like this but with sosa:isSampleOf*
      owl:propertyChainAxiom ( sosa:hasFeatureOfInterest sosa:isSampleOf )""" ;
  schema:domainIncludes sosa:Deployment ;
  schema:domainIncludes sosa:Execution ;
  schema:domainIncludes sosa:ExecutionCollection ;
  schema:rangeIncludes sosa:FeatureOfInterest ;
  rdfs:isDefinedBy sosa-common: .

sosa:inputValueForExecution 
  a owl:ObjectProperty ;
  rdfs:label "input value for execution"@en ;
  skos:definition """
  relation from an InputValue to an Execution that used it
  """@en ;
  schema:rangeIncludes sosa:Execution ;
  owl:inverseOf sosa:hasInputValue ;
  rdfs:isDefinedBy sosa-common: .

sosa:isResultOf 
  a owl:ObjectProperty ;
  rdfs:label "is result of"@en ;
  skos:definition """
  relation from a result to the Execution that created or caused it
  """@en ;
  schema:rangeIncludes sosa:Execution ;
  owl:inverseOf sosa:hasResult ;
  rdfs:isDefinedBy sosa-common: .

sosa:madeBySystem 
  a owl:ObjectProperty ;
  rdfs:label "made by system"@en ;
  skos:definition """
  relation from an Execution to the System that made it
  """@en ;
  skos:scopeNote """
  madeBySystem generalizes the madeByActuator, madeBySensor, and madeBySampler properties. 
  It appears in the ontology to support the description of a common pattern for executions and their properties. 

  madeBySystem MUST be considered to be abstract, so SHOULD NOT appear in data instances. 
  Applications can use concrete sub-properties of madeBySystem.
  """@en ;
  schema:domainIncludes sosa:Execution ;
  schema:domainIncludes sosa:ExecutionCollection ;
  schema:rangeIncludes sosa:System ;
  owl:inverseOf sosa:madeExecution ;
  rdfs:isDefinedBy sosa-common: .

sosa:phenomenonOccurred 
  a owl:ObjectProperty ;
  rdfs:label "phenomenon occurred"@en ;
  skos:definition """
  result of an Execution that this time applies to
  """@en ;
  schema:domainIncludes time:TemporalEntity ;
  schema:rangeIncludes sosa:Execution ;
  owl:inverseOf sosa:phenomenonTime ;
  rdfs:isDefinedBy sosa-common: .

sosa:phenomenonTime 
  a owl:ObjectProperty ;
  rdfs:label "phenomenon time"@en ;
  skos:definition """
  time that the result of an Execution applies to the subject entity

  It may be an interval or an instant, or some other compound temporal entity [[!owl-time]].
  """@en ;
  skos:scopeNote """
  The phenomenonTime is not necessarily the same as the resultTime. 
  
  In the case of Actuation, phenomenonTime SHOULD indicate the time during which the actuator was active. 

  In the case of Observation, the phenomenonTime MAY be distant from the resultTime. 
  For example in the case of forecasts the phenomenonTime is after the resultTime. 
  In historical, geological and cosmological investigations the phenomenonTime can be far in the past, while the resultTime is contemporary. 

  In the case of Sampling the phenomenonTime SHOULD indicate the time during which the Sampling Procedure was active.
  The resultTime can indicate when the sample comes into the posession of the operator. 
  """@en ;
  schema:domainIncludes sosa:Execution ;
  schema:domainIncludes sosa:ExecutionCollection ;
  schema:rangeIncludes time:TemporalEntity ;
  owl:inverseOf sosa:phenomenonOccurred ;
  rdfs:isDefinedBy sosa-common: .

sosa:resultTime 
  a owl:DatatypeProperty ;
  rdfs:label "result time"@en ;
  skos:definition """
  instant of time when the Observation or Sampling was completed
  """@en ;
  rdfs:comment "The value would usually be encoded using xsd:dateTime xsd:date xsd:gYearMonth xsd:gYear"@en ;
  schema:domainIncludes sosa:Execution ;
  schema:domainIncludes sosa:ExecutionCollection ;
  rdfs:isDefinedBy sosa-common: .

sosa:startTime 
  a owl:DatatypeProperty ;
  rdfs:label "start time"@en ;
  skos:definition """
  instant of time when the Execution or ExecutionCollection or Deployment was initiated or tasked
  """@en ;
  rdfs:comment "The value would usually be encoded using xsd:dateTime xsd:date xsd:gYearMonth xsd:gYear"@en ;
  schema:domainIncludes sosa:Deployment ;
  schema:domainIncludes sosa:Execution ;
  schema:domainIncludes sosa:ExecutionCollection ;
  rdfs:isDefinedBy sosa-common: .

sosa:usedProcedure 
  a owl:ObjectProperty ;
  rdfs:label "used procedure"@en ;
  skos:definition """
  relation from an Execution or ExecutionCollection to a Procedure used to make it
  """@en ;
  schema:domainIncludes sosa:Execution ;
  schema:domainIncludes sosa:ExecutionCollection ;
  schema:rangeIncludes sosa:Procedure ;
  rdfs:isDefinedBy sosa-common: .

## Systems

sosa:Deployment 
  a owl:Class ;
  rdfs:label "Deployment"@en ;
  skos:definition """
  arrangement of one or more assets (Systems and/or Platforms) to execute Procedures,
  usually with respect to a designated subject entity (FeatureOfInterest)
  """@en ;
  skos:note """
  A Deployment will usually be for a specified time interval. 
  It MAY involve Platforms, or Systems, or both. 
  A Deployment can be used quite flexibly to describe the use of systems, and platforms that host systems, with respect to a feature of interest. 
  """@en ;
  skos:example "For example, a temperature Sensor deployed on a wall, or a whole network of Sensors deployed for an Observation campaign."@en ;
  rdfs:isDefinedBy sosa-common: .

sosa:Platform 
  a owl:Class ;
  rdfs:label "Platform or Host"@en ;
  skos:prefLabel "Platform" ;
  skos:altLabel "Host" ;
  skos:definition """
  entity that hosts other entities, particularly Systems and other Platforms
  """@en ;
  skos:scopeNote "The INSPIRE 'Environmental Monitoring Facility' may be implemented using SOSA by the OWL/RDFS class 'Platform'" ;
  dcterms:source <https://inspire.ec.europa.eu/id/document/tg/ef> ;
  skos:example """A post, buoy, vehicle, ship, aircraft, satellite, cell-phone, human or animal may act as platforms for (technical or biological) sensors or actuators.
  An environmental monitoring facility. 
  A platform that hosts a set of sensors. 
  A team performing a survey, where each team member would be modeled as an Observer."""@en ;
  rdfs:isDefinedBy sosa-common: .

sosa:System 
  a owl:Class ;
  rdfs:label "System"@en ;
  skos:definition """
  entity that implements a Procedure in the context of an Execution
  """@en ; 
  skos:note """
  This may be a device, a piece of infrastructure, an agent (including humans), or software (simulation).

  Different Systems can implement the same (reusable) Procedure for different Executions.

  A System may have components, its sub-systems, which are other systems.
  """@en ;
  skos:scopeNote """
  System generalizes the Actuator, Sensor, and Sampler classes. 
  It appears in the ontology to support the description of a common pattern for executions and their properties. 

  System MUST be considered to be abstract, so any individual System SHOULD be declared to be an instance of one of the concrete sub-classes, and not of the System class. 
  """@en ;
  skos:scopeNote """
  Specific system types may be implemented as sub-classes of this class or its sub-classes.
  Their descriptions may capture the properties and characteristics of a whole class of systems, corresponding with the information typically found in a data-sheet.

  Individual system instances are members of this class or its sub-classes. 
  """@en ;
  skos:scopeNote """
  The association of a System (Actuator, Sensor, and Sampler) with a FeatureOfInterest is usually in the context of an Execution or a Deployment. 

  A System can be hosted by a Platform. 

  A System can be deployed for a specified time interval as part of a Deployment.
  """@en ;
  rdfs:isDefinedBy sosa-common: .

sosa:deployedAsset 
  a owl:ObjectProperty ;
  rdfs:label "deployed asset"@en ;
  skos:definition """
  relation from a Deployment to an asset (System or Platform)
  """@en ;
  schema:domainIncludes sosa:Deployment ;
  schema:rangeIncludes sosa:Platform ;
  schema:rangeIncludes sosa:System ;
  rdfs:isDefinedBy sosa-common: .

sosa:deployedOnPlatform 
  a owl:ObjectProperty ;
  rdfs:label "deployed on platform"@en ;
  skos:definition """
  relation from a Deployment to a Platform on which Systems are hosted
  """@en ;
  schema:domainIncludes sosa:Deployment ;
  schema:rangeIncludes sosa:Platform ;
  owl:inverseOf sosa:inDeployment ;
  rdfs:isDefinedBy sosa-common: .

sosa:deployedSystem 
  a owl:ObjectProperty ;
  rdfs:label "deployed system"@en ;
  skos:definition """
  relation from a Deployment to a deployed System
  """@en ;
  schema:domainIncludes sosa:Deployment ;
  schema:rangeIncludes sosa:System ;
  owl:inverseOf sosa:hasDeployment ;
  rdfs:isDefinedBy sosa-common: .

sosa:hasDeployment 
  a owl:ObjectProperty ;
  rdfs:label "has deployment"@en ;
  skos:definition """
  relation from a System to a Deployment in which it is deployed
  """@en ;
  schema:domainIncludes sosa:System ;
  schema:domainIncludes sosa:Platform ;
  schema:rangeIncludes sosa:Deployment ;
  owl:inverseOf sosa:deployedSystem ;
  rdfs:isDefinedBy sosa-common: .

sosa:hasSubSystem 
  a owl:ObjectProperty ;
  rdfs:label "has subsystem"@en ;
  skos:definition """
  relation from a System to a component System
  """@en ;
  schema:domainIncludes sosa:System ;
  schema:rangeIncludes sosa:System ;
  owl:inverseOf sosa:isSubSystemOf ;
  rdfs:isDefinedBy sosa-common: .

sosa:hosts 
  a owl:ObjectProperty ;
  rdfs:label "hosts"@en ;
  skos:definition """
  relation from a Platform to an asset (System or Platform) hosted or mounted on it
  """@en ;
  schema:domainIncludes sosa:Platform ;
  schema:rangeIncludes sosa:Platform ;
  schema:rangeIncludes sosa:System ;
  owl:inverseOf sosa:isHostedBy ;
  rdfs:isDefinedBy sosa-common: .

sosa:implements 
  a owl:ObjectProperty ;
  rdfs:label "implements"@en ;
  skos:definition """
  relation from a System to the Procedure that it is capable of executing
  """@en ;
  skos:example "For example, the relationship between a sensor and the scientific measuring Procedure via which it senses."@en ;
  schema:domainIncludes sosa:System ;
  schema:rangeIncludes sosa:Procedure ;
  owl:inverseOf sosa:implementedBy ;
  rdfs:isDefinedBy sosa-common: .

sosa:inDeployment 
  a owl:ObjectProperty ;
  rdfs:label "in deployment"@en ;
  skos:definition """
  relation from a Platform to a Deployment
  """@en ;
  skos:example "For example, a relation between a buoy and a deployment of several Sensors."@en ;
  schema:domainIncludes sosa:Platform ;
  schema:rangeIncludes sosa:Deployment ;
  owl:inverseOf sosa:deployedOnPlatform ;
  rdfs:isDefinedBy sosa-common: .

sosa:isHostedBy 
  a owl:ObjectProperty ;
  rdfs:label "is hosted by"@en ;
  skos:definition """
  relation from an asset (System or Platform), to a Platform that it is mounted on or hosted by
  """@en ;
  schema:domainIncludes sosa:System ;
  schema:domainIncludes sosa:Platform ;
  schema:rangeIncludes sosa:Platform ;
  owl:inverseOf sosa:hosts ;
  rdfs:isDefinedBy sosa-common: .

sosa:isSubSystemOf 
  a owl:ObjectProperty ;
  rdfs:label "is subsystem of"@en ;
  skos:definition """
  relation from a component System to a System that it belongs to
  """@en ;
  schema:domainIncludes sosa:System ;
  schema:rangeIncludes sosa:System ;
  owl:inverseOf sosa:hasSubSystem ;
  rdfs:isDefinedBy sosa-common: .

sosa:madeExecution 
  a owl:ObjectProperty ;
  rdfs:label "made execution"@en ;
  skos:definition """
  relation from a System to an Execution or ExecutionCollection that it has made
  """@en ;
  skos:scopeNote """
  madeExecution generalizes the madeActuation, madeObservation, and madeSampling properties. 
  It appears in the ontology to support the description of a common pattern for executions and their properties. 

  madeExecution MUST be considered to be abstract, so SHOULD NOT appear in data instances. 
  Applications can use concrete sub-properties of madeExecution.
  """@en ;
  schema:domainIncludes sosa:System ;
  schema:rangeIncludes sosa:Execution ;
  schema:rangeIncludes sosa:ExecutionCollection ;
  owl:inverseOf sosa:madeBySystem ;
  rdfs:isDefinedBy sosa-common: .

## Utility terms 

sosa:hasMember 
  a owl:ObjectProperty ;
  rdfs:label "has member of collection" ;
  skos:definition """
  link from a Collection to an Execution or Sample or Collection of these that is part of it
  """ ;
  skos:scopeNote "rules for the consistency of values of properties of collections and properties of their members are given for each collection type" ;
  skos:editorialNote "Note that there is a single `member` property. OWL or SHACL constraints may limit the range depending on the context of different collection types" ;
  schema:domainIncludes sosa:ExecutionCollection ;
  schema:domainIncludes sosa:SampleCollection ;
  schema:rangeIncludes sosa:Execution ;
  schema:rangeIncludes sosa:Sample ;
  schema:rangeIncludes sosa:ExecutionCollection ;
  schema:rangeIncludes sosa:SampleCollection ;
  owl:inverseOf sosa:isMemberOf ;
  rdfs:isDefinedBy sosa-common: .

sosa:isMemberOf 
  a owl:ObjectProperty ;
  rdfs:label "is member of collection" ;
  skos:definition """
  link from an Execution or Sample or Collection of these, to a collection that it is part of
  """ ;
  skos:scopeNote "rules for the consistency of values of properties of collections and properties of their members are given for each collection type" ;
  skos:editorialNote "Note that there is a single `member` property. OWL or SHACL constraints may limit the range depending on the context of different collection types" ;
  schema:domainIncludes sosa:Execution ; 
  schema:domainIncludes sosa:Sample ;
  schema:domainIncludes sosa:ExecutionCollection ;
  schema:domainIncludes sosa:SampleCollection ;
  schema:rangeIncludes sosa:ExecutionCollection ;
  schema:rangeIncludes sosa:SampleCollection ;
  owl:inverseOf sosa:hasMember ;
  rdfs:isDefinedBy sosa-common: .


